theories/channel/channel.v
@@ -27,8 +27,8 @@ protocols. *)
 From iris.heap_lang Require Import proofmode notation.
 From iris.heap_lang.lib Require Import spin_lock.
 From iris.heap_lang Require Import lifting.
-From iris.algebra Require Import excl auth list.
-From actris.utils Require Import auth_excl llist.
+From iris.algebra Require Import excl_auth list.
+From actris.utils Require Import llist.
 Set Default Proof Using "Type".
 
 Inductive side := Left | Right.
@@ -70,10 +70,10 @@ Definition recv : val :=
 (** * Setup of Iris's cameras *)
 Class chanG Σ := {
   chanG_lockG :> lockG Σ;
-  chanG_authG :> auth_exclG (listO valO) Σ;
+  chanG_authG :> inG Σ (excl_authR (listO valO));
 }.
 Definition chanΣ : gFunctors :=
-  #[ lockΣ; auth_exclΣ (constOF (listO valO)) ].
+  #[ lockΣ; GFunctor (excl_authR (listO valO)) ].
 Instance subG_chanΣ {Σ} : subG chanΣ Σ → chanG Σ.
 Proof. solve_inG. Qed.
 
@@ -89,8 +89,8 @@ Section channel.
   (** * The logical connectives *)
   Definition chan_inv (γ : chan_name) (l r : loc) : iProp Σ :=
     (∃ ls rs,
-      llist sbi_internal_eq l ls ∗ own (chan_l_name γ) (● to_auth_excl ls) ∗
-      llist sbi_internal_eq r rs ∗ own (chan_r_name γ) (● to_auth_excl rs))%I.
+      llist sbi_internal_eq l ls ∗ own (chan_l_name γ) (●E ls) ∗
+      llist sbi_internal_eq r rs ∗ own (chan_r_name γ) (●E rs))%I.
   Typeclasses Opaque chan_inv.
 
   Definition is_chan (γ : chan_name) (c1 c2 : val) : iProp Σ :=
@@ -104,16 +104,16 @@ Section channel.
   Lemma chan_inv_alt s γ l r :
     chan_inv γ l r ⊣⊢ ∃ ls rs,
       llist sbi_internal_eq (side_elim s l r) ls ∗
-      own (side_elim s chan_l_name chan_r_name γ) (● to_auth_excl ls) ∗
+      own (side_elim s chan_l_name chan_r_name γ) (●E ls) ∗
       llist sbi_internal_eq (side_elim s r l) rs ∗
-      own (side_elim s chan_r_name chan_l_name γ) (● to_auth_excl rs).
+      own (side_elim s chan_r_name chan_l_name γ) (●E rs).
   Proof.
     destruct s; rewrite /chan_inv //=.
     iSplit; iDestruct 1 as (ls rs) "(?&?&?&?)"; iExists rs, ls; iFrame.
   Qed.
 
   Definition chan_own (γ : chan_name) (s : side) (vs : list val) : iProp Σ :=
-    own (side_elim s chan_l_name chan_r_name γ) (◯ to_auth_excl vs)%I.
+    own (side_elim s chan_l_name chan_r_name γ) (◯E vs)%I.
 
   (** * The proof rules *)
   Global Instance chan_own_timeless γ s vs : Timeless (chan_own γ s vs).
@@ -128,13 +128,13 @@ Section channel.
     wp_lam.
     wp_apply (lnil_spec with "[//]"); iIntros (l) "Hl".
     wp_apply (lnil_spec with "[//]"); iIntros (r) "Hr".
-    iMod (own_alloc (● (to_auth_excl []) ⋅ ◯ (to_auth_excl []))) as (lsγ) "[Hls Hls']".
-    { by apply auth_both_valid. }
-    iMod (own_alloc (● (to_auth_excl []) ⋅ ◯ (to_auth_excl []))) as (rsγ) "[Hrs Hrs']".
-    { by apply auth_both_valid. }
+    iMod (own_alloc (●E [] ⋅ ◯E [])) as (lsγ) "[Hls Hls']".
+    { by apply excl_auth_valid. }
+    iMod (own_alloc (●E [] ⋅ ◯E [])) as (rsγ) "[Hrs Hrs']".
+    { by apply excl_auth_valid. }
     wp_apply (newlock_spec N (∃ ls rs,
-      llist sbi_internal_eq l ls ∗ own lsγ (● to_auth_excl ls) ∗
-      llist sbi_internal_eq r rs ∗ own rsγ (● to_auth_excl rs))%I with "[Hl Hr Hls Hrs]").
+      llist sbi_internal_eq l ls ∗ own lsγ (●E ls) ∗
+      llist sbi_internal_eq r rs ∗ own rsγ (●E rs))%I with "[Hl Hr Hls Hrs]").
     { eauto 10 with iFrame. }
     iIntros (lk γlk) "#Hlk". wp_pures.
     iApply ("HΦ" $! _ _ (Chan_name γlk lsγ rsγ)); simpl.
@@ -157,8 +157,9 @@ Section channel.
       (vs ws) "(Hll & Hvs & Href' & Hws)".
     wp_seq. wp_bind (Fst (_,_)%V)%E.
     iMod "HΦ" as (vs') "[Hchan HΦ]".
-    iDestruct (excl_eq with "Hvs Hchan") as %<-%leibniz_equiv.
-    iMod (excl_update _ _ _ (vs ++ [v]) with "Hvs Hchan") as "[Hvs Hchan]".
+    iDestruct (own_valid_2 with "Hvs Hchan") as %<-%excl_auth_agreeL.
+    iMod (own_update_2 _ _ _ (●E (vs ++ [v]) ⋅ _) with "Hvs Hchan") as "[Hvs Hchan]".
+    { apply excl_auth_update. }
     wp_pures. iMod ("HΦ" with "Hchan") as "HΦ"; iModIntro.
     wp_apply (lsnoc_spec with "[$Hll //]"); iIntros "Hll".
     wp_apply (release_spec with "[-HΦ $Hlock $Hlocked]"); last eauto.
@@ -190,8 +191,9 @@ Section channel.
         rewrite /llist. eauto 10 with iFrame. }
       iIntros (_). by wp_pures.
     - iDestruct "HΦ" as "[_ >HΦ]". iDestruct "HΦ" as (vs') "[Hvs' HΦ]".
-      iDestruct (excl_eq with "Hvs Hvs'") as %<-%leibniz_equiv.
-      iMod (excl_update _ _ _ vs with "Hvs Hvs'") as "[Hvs Hvs']".
+      iDestruct (own_valid_2 with "Hvs Hvs'") as %<-%excl_auth_agreeL.
+      iMod (own_update_2 _ _ _ (●E vs ⋅ _) with "Hvs Hvs'") as "[Hvs Hvs']".
+      { apply excl_auth_update. }
       wp_pures. iMod ("HΦ" with "[//] Hvs'") as "HΦ"; iModIntro.
       wp_apply (lisnil_spec with "Hll"); iIntros "Hll". iMod "HΦ".
       wp_apply (lpop_spec with "Hll"); iIntros (v') "[% Hll]"; simplify_eq/=.
